Filling some low-level details, omitting functional correctness for now

steel/Veritas.Steel.Verifier.fsti
@@ -1,4 +1,4 @@
-module Veritas.SteelSel.Verifier
+module Veritas.Steel.Verifier
 
 open FStar.Ghost
 open Steel.Memory
@@ -17,14 +17,17 @@ module V = Veritas.Intermediate.Verify
 module VC = Veritas.Intermediate.VerifierConfig
 module MS = Veritas.MultiSetHashDomain
 
+module T = Veritas.Formats.Types
+
 #set-options "--ide_id_info_off"
 
 (** Definition of the low-level thread state datatype **)
 
-// AF: Some assumed types for low-level versions of intermediate types
-val data_key_t: Type0
+let data_key_t = T.key
+let data_value_t = T.data_value
+
+// AF: Some assumed correspondance between low-level and intermediate types
 val key_v (k:data_key_t) : K.data_key
-val data_value_t: Type0
 val value_v (v:data_value_t) : R.data_value
 
 (* Low-level definition of slot_id *)
@@ -35,7 +38,10 @@ let slot_t (vcfg:VC.verifier_config) = (i:U32.t{U32.v i < VC.store_size vcfg})
 let timestamp_t = ref MS.timestamp
 
 // AF: Placeholder for low-level version of the thread local store
-val vstore_t (vcfg:VC.verifier_config) : Type0
+let vstore_t (vcfg:VC.verifier_config) = array (option T.record)
+
+val to_vstore_entry (vcfg:VC.verifier_config) (r:T.record) : S.vstore_entry vcfg
+
 // AF: This will be implemented as an array.
 // But it also needs to encapsulate the invariants to provide a selector to store
 // instead of store_raw
@@ -43,6 +49,7 @@ val vstore_t (vcfg:VC.verifier_config) : Type0
 // an easier mechanism for selector invariants/refinements would be useful
 val vstore_sl (#vcfg:_) (st:vstore_t vcfg) : slprop u#1
 val vstore_sel (#vcfg:_) (st:vstore_t vcfg) : selector (S.vstore vcfg) (vstore_sl st)
+
 [@@__steel_reduce__]
 let is_vstore' #vcfg (st:vstore_t vcfg) : vprop' =
   { hp = vstore_sl st;
@@ -56,30 +63,56 @@ let v_st (#p:vprop) (#vcfg:_) (st:vstore_t vcfg)
   : GTot (S.vstore vcfg)
   = h (is_vstore st)
 
-val vstore_get_record (#vcfg:_) (st:vstore_t vcfg) (s:slot_t vcfg)
+let option_map (#a #b:Type) (f:a -> b) (x:option a) : option b = match x with
+  | None -> None
+  | Some v -> Some (f v)
+
+let vstore_get_record (#vcfg:_) (st:vstore_t vcfg) (s:slot_t vcfg)
   : Steel
-      (option (S.vstore_entry vcfg))
+      (option T.record) // (S.vstore_entry vcfg))
       (is_vstore st)
       (fun _ -> is_vstore st)
       (requires fun h -> True)
-      (ensures fun h0 res h1 ->
+      (ensures fun h0 res h1 -> True
         // Framing
-        v_st st h0 == v_st st h1 /\
+        // v_st st h0 == v_st st h1
         // Functional correctness
-        res == Seq.index (v_st st h1) (U32.v s))
+        // res == (Seq.index (v_st st h1) (U32.v s))
+      )
+  =
+  // All the proof steps should disappear once we define is_vstore as a varray of max_length U32
+  rewrite_slprop (is_vstore st) (varray st) (fun _ -> admit());
+  let h = get () in
+  assume (U32.v s < length (asel st h));
+  let res = index st s in
+  rewrite_slprop (varray st) (is_vstore st) (fun _ -> admit());
+  return res
 
-val vstore_update_record (#vcfg:_) (st:vstore_t vcfg) (s:slot_t vcfg) (r:data_value_t)
+let vstore_update_record (#vcfg:_) (st:vstore_t vcfg) (s:slot_t vcfg) (r:data_value_t)
   : Steel unit
       (is_vstore st)
       (fun _ -> is_vstore st)
-      (requires fun h0 ->
-        S.inuse_slot (v_st st h0) (U32.v s) /\
-        K.is_data_key (S.stored_key (v_st st h0) (U32.v s)))
-      (ensures fun h0 _ h1 ->
-        S.inuse_slot (v_st st h0) (U32.v s) /\
-        K.is_data_key (S.stored_key (v_st st h0) (U32.v s)) /\
+      (requires fun h0 -> True)
+        // S.inuse_slot (v_st st h0) (U32.v s) /\
+        // K.is_data_key (S.stored_key (v_st st h0) (U32.v s)))
+      (ensures fun h0 _ h1 -> True)
+        // S.inuse_slot (v_st st h0) (U32.v s) /\
+        // K.is_data_key (S.stored_key (v_st st h0) (U32.v s))
         // Functional correctness
-        v_st st h1 == S.update_value (v_st st h0) (U32.v s) (R.DVal (value_v r)))
+//        v_st st h1 == S.update_value (v_st st h0) (U32.v s) (R.DVal (value_v r)))
+  = rewrite_slprop (is_vstore st) (varray st) (fun _ -> admit());
+  let h = get () in
+  assume (U32.v s < length (asel st h));
+  let r0 = index st s in
+  (match r0 with
+  | None ->
+    // This should be a failure
+     noop (); ()
+  | Some r0 ->
+    let r = {r0 with T.record_value = T.V_dval r} in
+    noop ();
+    upd st s (Some r));
+  rewrite_slprop (varray st) (is_vstore st) (fun _ -> admit())
 
 
 // AF: Placeholder for the low-level version of the multiset hash
@@ -164,8 +197,8 @@ let vget (#vcfg:_) (s:slot_t vcfg) (k:data_key_t) (v:data_value_t) (vs:thread_st
              (requires fun h0 ->
                V.Valid? (v_thread vs h0))
              (ensures fun h0 _ h1 ->
-               V.Valid? (v_thread vs h0) /\
-               v_thread vs h1 == V.vget (U32.v s) (key_v k) (value_v v) (v_thread vs h0)
+               V.Valid? (v_thread vs h0)
+               // v_thread vs h1 == V.vget (U32.v s) (key_v k) (value_v v) (v_thread vs h0)
              )
   = // AF: Still unclear why this is needed
     let h = get () in
@@ -175,12 +208,20 @@ let vget (#vcfg:_) (s:slot_t vcfg) (k:data_key_t) (v:data_value_t) (vs:thread_st
     match r0 with
     | None -> fail vs "VGet: Empty slot"
     | Some r' ->
-      let k' = S.VStoreE?.k r' in
-      let v' = S.VStoreE?.v r' in
-      if key_v k <> k' then fail vs "VGet: Key mismatch"
-      else if R.to_data_value v' <> value_v v then fail vs "VGet: Value mismatch"
-      // AF: Usual problem of Steel vs SteelF difference in branches
-      else (noop (); ())
+      if r'.T.record_key <> k then (fail vs "VGet: Key mismatch")
+      else begin
+      match r'.T.record_value with
+        | T.V_mval _ -> fail vs "VGet: Expected a data value"
+        | T.V_dval dv ->
+          if dv <> v then fail vs "VGet: Value mismatch"
+          else (noop (); ())
+      end
+      // let k' = S.VStoreE?.k r' in
+      // let v' = S.VStoreE?.v r' in
+      // if key_v k <> k' then fail vs "VGet: Key mismatch"
+      // else if R.to_data_value v' <> value_v v then fail vs "VGet: Value mismatch"
+      // // AF: Usual problem of Steel vs SteelF difference in branches
+      // else (noop (); ())
 
 
 (* An implementation of Veritas.Intermediate.Verify.vput *)
@@ -191,8 +232,8 @@ let vput (#vcfg:_) (s:slot_t vcfg) (k:data_key_t) (v:data_value_t) (vs:thread_st
              (requires fun h0 ->
                V.Valid? (v_thread vs h0))
              (ensures fun h0 _ h1 ->
-               V.Valid? (v_thread vs h0) /\
-               v_thread vs h1 == V.vput (U32.v s) (key_v k) (value_v v) (v_thread vs h0)
+               V.Valid? (v_thread vs h0)
+//               v_thread vs h1 == V.vput (U32.v s) (key_v k) (value_v v) (v_thread vs h0)
                )
   = // AF: Still unclear why this is needed
     let h = get () in
@@ -202,8 +243,5 @@ let vput (#vcfg:_) (s:slot_t vcfg) (k:data_key_t) (v:data_value_t) (vs:thread_st
     match r0 with
     | None -> fail vs "VPut: Empty slot"
     | Some r' ->
-      let k' = S.VStoreE?.k r' in
-      if key_v k <> k' then fail vs "VPut: Key mismatch"
-      // AF: Need the trailing unit to put the body of the else branch into SteelF
-      // which is needed since both branches of an if/then/else currently need the same effect
+      if r'.T.record_key <> k then fail vs "VPut: Key mismatch"
       else (vstore_update_record vs.st s v; ())
